port over rest of cryptoffi

new/proof/github_com/sanjit_bhat/pav/cryptoffi.v
@@ -40,12 +40,10 @@ relative to the crypto model, it says the inputs are in the set of hashes. *)
 Definition is_hash (data : option (list w8)) (hash : list w8) : iProp Σ.
 Proof. Admitted.
 
-#[global]
-Instance is_hash_persistent data hash : Persistent (is_hash data hash).
+#[global] Instance is_hash_pers data hash : Persistent (is_hash data hash).
 Proof. Admitted.
 
-#[global]
-Instance is_hash_timeless data hash : Timeless (is_hash data hash).
+#[global] Instance is_hash_timeless data hash : Timeless (is_hash data hash).
 Proof. Admitted.
 
 Lemma is_hash_det data hash0 hash1 :
@@ -110,6 +108,231 @@ Lemma wp_Hasher_Sum sl_b_in hr data b_in :
     "Hown_hr" ∷ own_Hasher hr data ∗
     "Hsl_b_out" ∷ sl_b_out ↦* (b_in ++ hash) ∗
     "#His_hash" ∷ is_hash (Some data) hash
+  }}}.
+Proof. Admitted.
+
+(* Signatures. *)
+
+(* is_sig_sk says that an sk is in-distribution.
+furthermore, it came from calling the Generate fn,
+and the underlying sk is enclosed in the ffi,
+forcing all users to establish the sigpred.
+pk is a mathematical list so it can leave the ffi and be sent
+between parties. *)
+Definition is_sig_sk (ptr_sk : loc) (pk : list w8) (P : list w8 → iProp Σ) : iProp Σ.
+Admitted.
+
+#[global] Instance is_sig_sk_pers ptr_sk pk P :
+  Persistent (is_sig_sk ptr_sk pk P).
+Proof. Admitted.
+
+(* is_sig_pk says that pk is in-distribution.
+also, that it came from the Generate fn,
+tied by P to a corresponding sk in the ffi. *)
+Definition is_sig_pk (pk : list w8) (P : list w8 → iProp Σ) : iProp Σ.
+Admitted.
+
+#[global] Instance is_sig_pk_pers pk P : Persistent (is_sig_pk pk P).
+Proof. Admitted.
+
+Lemma is_sig_sk_to_pk ptr_sk pk P : is_sig_sk ptr_sk pk P -∗ is_sig_pk pk P.
+Proof. Admitted.
+
+(* is_sig says that Verify will ret True on these inputs.
+relative to the crypto model, it says the inputs are in the set of
+memoized=True Verify inputs. *)
+Definition is_sig (pk msg sig : list w8) : iProp Σ.
+Admitted.
+
+#[global] Instance is_sig_pers pk msg sig : Persistent (is_sig pk msg sig).
+Proof. Admitted.
+
+(* the proof for is_sig_to_pred splits into two cases:
+1) the sig came from sign. P clearly holds.
+2) an adversary forged the sig.
+EUF-CMA guarantees that this only happens if the genuine key holder
+signed the same msg in the past. P holds from the orig signing op. *)
+Lemma is_sig_to_pred pk P msg sig :
+  is_sig_pk pk P -∗ is_sig pk msg sig -∗ P msg.
+Proof. Admitted.
+
+Lemma wp_SigGenerateKey P :
+  (∀ l, Persistent (P l)) →
+  {{{ True }}}
+  @! cryptoffi.SigGenerateKey #()
+  {{{
+    sl_pk pk ptr_sk, RET (#sl_pk, #ptr_sk);
+    "Hsl_sig_pk" ∷ sl_pk ↦* pk ∗
+    "#His_sig_pk" ∷ is_sig_pk pk P ∗
+    "#His_sig_sk" ∷ is_sig_sk ptr_sk pk P
+ }}}.
+Proof. Admitted.
+
+Lemma wp_SigPrivateKey_Sign ptr_sk pk P sl_msg msg d0 :
+  {{{
+    "#His_sig_sk" ∷ is_sig_sk ptr_sk pk P ∗
+    "HP" ∷ P msg ∗
+    "Hsl_msg" ∷ sl_msg ↦*{d0} msg
+  }}}
+  ptr_sk @ (ptrT.id cryptoffi.SigPrivateKey.id) @ "Sign" #sl_msg
+  {{{
+    sl_sig (sig : list w8), RET #sl_sig;
+    "Hsl_msg" ∷ sl_msg ↦*{d0} msg ∗
+    "Hsl_sig" ∷ sl_sig ↦* sig ∗
+    "#His_sig" ∷ is_sig pk msg sig
+  }}}.
+Proof. Admitted.
+
+Lemma wp_SigPublicKey_Verify sl_pk pk sl_sig sl_msg (sig msg : list w8) d0 d1 d2 :
+  {{{
+    "Hsl_sig_pk" ∷ sl_pk ↦*{d0} pk ∗
+    "Hsl_msg" ∷ sl_msg ↦*{d1} msg ∗
+    "Hsl_sig" ∷ sl_sig ↦*{d2} sig
+  }}}
+  sl_pk @ (ptrT.id cryptoffi.SigPublicKey.id) @ "Verify" #sl_msg #sl_sig
+  {{{
+    (err : bool), RET #err;
+    "Hsl_sig_pk" ∷ sl_pk ↦*{d0} pk ∗
+    "Hsl_msg" ∷ sl_msg ↦*{d1} msg ∗
+    "Hsl_sig" ∷ sl_sig ↦*{d2} sig ∗
+    "Hgenie" ∷
+      match err with
+      | true => ¬ is_sig pk msg sig
+      | false =>
+        "#His_sig" ∷ is_sig pk msg sig
+      end
+  }}}.
+Proof. Admitted.
+
+(* Verifiable Random Functions (VRFs).
+IETF spec: https://www.rfc-editor.org/rfc/rfc9381.html.
+we model correctness (is_vrf_proof), "Full Uniqueness" (is_vrf_out_det),
+and "Full Collision Resistance" (is_vrf_out_inj). *)
+
+(* is_vrf_sk provides ownership of an sk from the VrfGenerateKey function. *)
+Definition is_vrf_sk (ptr_sk : loc) (pk : list w8) : iProp Σ.
+Admitted.
+
+#[global] Instance is_vrf_sk_pers ptr_sk pk : Persistent (is_vrf_sk ptr_sk pk).
+Proof. Admitted.
+
+(* is_vrf_pk says that pk satisfies certain mathematical crypto checks.
+this is in contrast to is_sig_pk, which additionally says that
+the corresponding sk never left the ffi. *)
+Definition is_vrf_pk (ptr_pk : loc) (pk : list w8) : iProp Σ.
+Admitted.
+
+#[global] Instance is_vrf_pk_pers ptr_pk pk : Persistent (is_vrf_pk ptr_pk pk).
+Proof. Admitted.
+
+(* is_vrf_proof helps model correctness.
+i.e., a caller gets this from Prove / Verify,
+and uses it to prove that Verify should not return an error. *)
+Definition is_vrf_proof (pk data proof : list w8) : iProp Σ.
+Admitted.
+
+#[global] Instance is_vrf_proof_pers pk data proof :
+  Persistent (is_vrf_proof pk data proof).
+Proof. Admitted.
+
+(* is_vrf_out gets returned from Prove / Verify and abstracts out
+the specific proof associated with a VRF computation.
+this is convenient because the spec does not rule out multiple proofs
+between the same pk, data, and output. *)
+Definition is_vrf_out (pk data out : list w8) : iProp Σ.
+Admitted.
+
+#[global] Instance is_vrf_out_pers pk data out :
+  Persistent (is_vrf_out pk data out).
+Proof. Admitted.
+
+(* is_vrf_out_det models "Full Uniqueness".
+this always holds for ECVRF. *)
+Lemma is_vrf_out_det pk data out0 out1 :
+  is_vrf_out pk data out0 -∗ is_vrf_out pk data out1 -∗ ⌜ out0 = out1⌝.
+Proof. Admitted.
+
+(* is_vrf_out_inj models "Full Collision Resistance".
+"Full" (as opposed to "Trusted") holds for ECVRF as long
+as the `validate_key` parameter to `ECVRF_verify` is true.
+key validation is done when running `VrfPublicKeyDecode`
+on an adversarially-provided pk. *)
+Lemma is_vrf_out_inj pk data0 data1 out :
+  is_vrf_out pk data0 out -∗ is_vrf_out pk data1 out -∗ ⌜ data0 = data1 ⌝.
+Proof. Admitted.
+
+Lemma is_vrf_out_len pk data out :
+  is_vrf_out pk data out -∗ ⌜ Z.of_nat (length out) = hash_len ⌝.
+Proof. Admitted.
+
+Lemma wp_VrfGenerateKey :
+  {{{ True }}}
+  @! cryptoffi.VrfGenerateKey #()
+  {{{
+    (ptr_pk ptr_sk : loc) (pk : list w8), RET (#ptr_pk, #ptr_sk);
+    "#His_vrf_pk" ∷ is_vrf_pk ptr_pk pk ∗
+    "#His_vrf_sk" ∷ is_vrf_sk ptr_sk pk
+  }}}.
+Proof. Admitted.
+
+Lemma wp_VrfPrivateKey_Prove ptr_sk pk sl_data (data : list w8) d0 :
+  {{{
+    "#His_vrf_sk" ∷ is_vrf_sk ptr_sk pk ∗
+    "Hsl_data" ∷ sl_data ↦*{d0} data
+  }}}
+  ptr_sk @ (ptrT.id cryptoffi.VrfPrivateKey.id) @ "Prove" #sl_data
+  {{{
+    sl_out sl_proof (out proof : list w8), RET (#sl_out, #sl_proof);
+    "Hsl_data" ∷ sl_data ↦*{d0} data ∗
+    "Hsl_out" ∷ sl_out ↦* out ∗
+    "Hsl_proof" ∷ sl_proof ↦* proof ∗
+    "#His_vrf_proof" ∷ is_vrf_proof pk data proof ∗
+    "#His_vrf_out" ∷ is_vrf_out pk data out
+  }}}.
+Proof. Admitted.
+
+Lemma wp_VrfPublicKey_Verify ptr_pk pk sl_data sl_proof (data proof : list w8) d0 d1 :
+  {{{
+    "#His_vrf_pk" ∷ is_vrf_pk ptr_pk pk ∗
+    "Hsl_data" ∷ sl_data ↦*{d0} data ∗
+    "Hsl_proof" ∷ sl_proof ↦*{d1} proof
+  }}}
+  ptr_pk @ (ptrT.id cryptoffi.VrfPublicKey.id) @ "Verify" #sl_data #sl_proof
+  {{{
+    sl_out (out : list w8) (err : bool), RET (#sl_out, #err);
+    "Hsl_data" ∷ sl_data ↦*{d0} data ∗
+    "Hsl_proof" ∷ sl_proof ↦*{d1} proof ∗
+    "Hsl_out" ∷ sl_out ↦* out ∗
+    "Hgenie" ∷
+      match err with
+      | true => ¬ is_vrf_proof pk data proof
+      | false =>
+        "#His_proof" ∷ is_vrf_proof pk data proof ∗
+        "#His_out" ∷ is_vrf_out pk data out
+      end
+  }}}.
+Proof. Admitted.
+
+Lemma wp_VrfPublicKeyEncode ptr_pk pk :
+  {{{
+    "#His_vrf_pk" ∷ is_vrf_pk ptr_pk pk
+  }}}
+  @! cryptoffi.VrfPublicKeyEncode #ptr_pk
+  {{{
+    sl_enc, RET #sl_enc;
+    "Hsl_enc" ∷ sl_enc ↦* pk
+  }}}.
+Proof. Admitted.
+
+Lemma wp_VrfPublicKeyDecode sl_enc pk d0 :
+  {{{
+    "Hsl_enc" ∷ sl_enc ↦*{d0} pk
+  }}}
+  @! cryptoffi.VrfPublicKeyDecode #sl_enc
+  {{{
+    (ptr_pk : loc), RET #ptr_pk;
+    "Hsl_enc" ∷ sl_enc ↦*{d0} pk ∗
+    "#His_vrf_pk" ∷ is_vrf_pk ptr_pk pk
   }}}.
 Proof. Admitted.
 
